src/PlutusIR/Semantics/Dynamic/Bigstep/Examples/IfThenElse.v
@@ -38,7 +38,7 @@ Definition Ty_int : ty := Ty_Builtin DefaultUniInteger.
 Definition int_and_int_to_int : ty := Ty_Fun Ty_int (Ty_Fun Ty_int Ty_int).
 
 Example test_ifThenElse : forall x y, exists k,
-  Apply (LamAbs x int_and_int_to_int (Apply (Apply (Var x) (constInt 17)) (constInt 3))) (Apply (TyInst (Apply (LamAbs y Ty_int (Builtin IfThenElse)) (constInt 666)) (Ty_Builtin DefaultUniInteger)) (Constant (Some' (ValueOf DefaultUniBool true)))) =[k]=> constInt 17.
+  Apply (LamAbs x int_and_int_to_int (Apply (Apply (Var x) (constInt 17)) (constInt 3))) (Apply (TyInst (Apply (LamAbs y Ty_int (Builtin IfThenElse)) (constInt 666)) (Ty_Builtin DefaultUniInteger)) (Constant (ValueOf DefaultUniBool true))) =[k]=> constInt 17.
 Proof with (eauto with hintdb__eval_no_error || (try solve [decide_neutral])).
   unfold constInt.
   intros.
