src/PlutusIR/Semantics/SemanticEquivalence/Contextual.v
@@ -8,7 +8,7 @@ Import ListNotations.
 
 
 Definition Term_Unit : term :=
-  Constant (@Some' valueOf DefaultUniUnit (@ValueOf DefaultUniUnit tt))
+  Constant (ValueOf DefaultUniUnit tt)
 .
 
 Definition Ty_Unit : ty :=
