src/PlutusIR/Transform/LetNonStrict.v
@@ -33,7 +33,7 @@ Definition Ty_Unit : ty :=
   Ty_Builtin DefaultUniUnit.
 
 Definition t_unit : term :=
-  Constant (PlutusIR.Some' (PlutusIR.ValueOf DefaultUniUnit tt)).
+  Constant (ValueOf DefaultUniUnit tt).
 
 Inductive let_non_strict (Γ : ctx) : term -> term -> Type :=
 
